src/examples/Kuiper.Array.VectorizedAccess.fst
@@ -27,11 +27,7 @@ let kpre
   : slprop =
   gpu_pts_to_slice a 
       (global_id bid tid * 4) (global_id bid tid * 4 + 4)
-      (slice s (global_id bid tid * 4) (global_id bid tid * 4 + 4)) **
-  pure (aligned 16 a /\ is_global_array a)
-
-let scale_fun (v:float) (s:seq float) (i:nat{ i < length s }) : float =
-  v `mul` (s @! i)
+      (slice s (global_id bid tid * 4) (global_id bid tid * 4 + 4))
 
 noextract
 let scale_seq (v : float) (s : seq float)
@@ -52,88 +48,12 @@ let kpost
   gpu_pts_to_slice a (global_id bid tid * 4) (global_id bid tid * 4 + 4)
       (scale_seq v (slice s (global_id bid tid * 4) (global_id bid tid * 4 + 4)))
 
-module T = FStar.Tactics
-let is_gpu_loc (#[T.exact (`0)]gpu_id) (l:loc_id) = gpu_of l == gpu_id_loc gpu_id
-
-open Kuiper.Seq.Common { seq_blit }
-atomic
-fn gpu_array_vec_cpy_dh_mine
-  (#et : Type u#0) {| sized et, has_vec_cpy et |}
-  (dst_arr : array et)
-  (dst_off : SZ.t)
-  (#src_sz : erased nat)
-  (src_arr : gpu_array et src_sz)
-  (src_off : SZ.t)
-  (#src_slice_i : erased nat)
-  (#src_slice_j : erased nat)
-  (#f : perm)
-  (#ss : erased (seq et))
-  (#ds : erased (seq et))
-  (#_ : squash (dst_off + chunk et <= Seq.length ds))
-  (#_ : squash (src_slice_i <= src_off /\ src_off + chunk et <= src_slice_j))
-  (#_ : squash (Seq.length ss == src_slice_j - src_slice_i))
-  preserves gpu
-  preserves gpu_pts_to_slice src_arr #f src_slice_i src_slice_j ss
-  requires  pure (aligned' 16 src_arr src_off)
-  requires  dst_arr |-> ds
-  ensures   exists* s. dst_arr |-> s ** pure (s == seq_blit ds dst_off ss (src_off - src_slice_i) (chunk et))
-{ gpu_array_vec_cpy_dh #et dst_arr dst_off #src_sz src_arr src_off #src_slice_i #src_slice_j #f #ss #ds; }
-
-atomic
-fn gpu_array_vec_cpy_hd_mine
-  (#et : Type u#0) {| sized et, has_vec_cpy et |}
-  (#dst_sz : erased nat)
-  (dst_arr : gpu_array et dst_sz)
-  (dst_off : SZ.t)
-  (#dst_slice_i : erased nat)
-  (#dst_slice_j : erased nat)
-  (src_arr : array et)
-  (src_off : SZ.t)
-  (#f : perm)
-  (#ss : erased (seq et))
-  (#ds : erased (seq et))
-  (#_ : squash (dst_slice_i <= dst_off /\ dst_off + chunk et <= dst_slice_j))
-  (#_ : squash (Seq.length ds == dst_slice_j - dst_slice_i))
-  (#_ : squash (src_off + chunk et <= Seq.length ss))
-  preserves gpu
-  preserves src_arr |-> Frac f ss
-  requires  pure (aligned' 16 dst_arr dst_off)
-  requires  gpu_pts_to_slice dst_arr dst_slice_i dst_slice_j ds
-  ensures   exists* s'. gpu_pts_to_slice dst_arr dst_slice_i dst_slice_j s' ** pure (s' == seq_blit ds (dst_off - dst_slice_i) ss src_off (chunk et))
-{
-  admit()
-}
-
-inline_for_extraction
-fn op_Array_Access
-        u#a (#t: Type u#a)
-        (a: array t)
-        (i: SZ.t)
-        (#p: perm)
-        (#s: Ghost.erased (Seq.seq t){SZ.v i < Seq.length s})
-  requires pts_to a #p s
-  returns  res : t
-  ensures  pts_to a #p s **
-           rewrites_to res (Seq.index s (SZ.v i))
-{ admit() }
-
-inline_for_extraction
-fn op_Array_Assignment
-        u#a (#t: Type u#a)
-        (a: array t)
-        (i: SZ.t)
-        (v: t)
-        (#s: Ghost.erased (Seq.seq t) {SZ.v i < Seq.length s})
-  requires pts_to a s
-  ensures  exists* s'. pts_to a s' ** pure (s' == Seq.upd s (SZ.v i) v)
-{ admit() }
-
 inline_for_extraction noextract
 fn kf
   (size:sz)
   (#s:erased (seq float) { len s == SZ.v size })
   (nblk : erased (natle max_blocks))
-  (a:gpu_array float size)
+  (a:gpu_array float size { aligned 16 a })
   (v : float)
   (nthr : sz{nthr*4 * nblk == SZ.v size})
   (bid : szlt nblk)
@@ -146,14 +66,13 @@ ensures
   gpu **
   kpost v size a s nblk nthr bid tid
 {
-//  open Pulse.Lib.Array;
-  // elim_on_gpu_array a;
+  open Pulse.Lib.Array;
   let global_idx = ((bid *^ nthr +^ tid) *^ 4sz); rewrite each ((SZ.v bid * SZ.v nthr + SZ.v tid) * 4) as SZ.v global_idx;
   with s0. assert (gpu_pts_to_slice a (SZ.v global_idx) (SZ.v global_idx + 4) s0);
 
   let mut local = [| zero #float #_; 4sz |];
 
-  gpu_array_vec_cpy_dh_mine local 0sz a global_idx;
+  gpu_array_vec_cpy_dh local 0sz a global_idx;
   
   with s1. assert (local |-> s1);
   assert (pure (Seq.equal #float s0 s1));
@@ -166,24 +85,13 @@ ensures
   with s2. assert (local |-> s2);
   assert (pure (Seq.equal #float s2 (scale_seq v s1)));
 
-  gpu_array_vec_cpy_hd_mine a global_idx local 0sz;
+  gpu_array_vec_cpy_hd a global_idx local 0sz;
 
   with s3.
     assert (gpu_pts_to_slice a (SZ.v global_idx) (SZ.v global_idx + 4) s3);
   assert (pure (Seq.equal s3 s2));
   assert (pure (Seq.equal s3 (scale_seq v s0)));
   rewrite each SZ.v global_idx as ((SZ.v bid * SZ.v nthr + SZ.v tid) * 4);
-}
-
-ghost
-fn fuse_on_placeless (q:slprop) {| placeless q |} #l #p ()
-requires on l p
-requires q
-ensures on l (p ** q)
-{ 
-  placeless_on_intro q l;
-  admit();
-  rewrite (on l p ** on l q) as on l (p ** q); 
 }
 
 fn hf (v : V.vec float)
@@ -199,9 +107,9 @@ fn hf (v : V.vec float)
   with s. assert v |-> s;
   assert (pure (Seq.equal s (slice s 0 4)));
   let two = add #float one one;
-  fuse_on_placeless (pure (aligned 16 a /\ is_global_array a)) ();
+  rewrite each (a |-> s) as (a |-> slice s 0 4);
 
-  launch_kernel_1 (kf 4sz #(slice s 0 4) 1 a two 1sz 0sz 0sz);
+  launch_kernel_1 (kf 4sz #s 1 a two 1sz 0sz 0sz);
 
   gpu_memcpy_device_to_host v a 4sz;
 
