src/examples/Kuiper.ArrayReversal.fst
@@ -330,7 +330,7 @@ inline_for_extraction noextract
 fn reverse
     (#ty:Type0)
     (size:sz { size > 0sz /\ size % 2sz == 0sz /\ SZ.v size < max_blocks })
-    (a:gpu_array ty size)
+    (a:gpu_array ty size { is_global_array a })
     (#s: erased (seq ty) { len s == SZ.v size })
   preserves
     cpu
