src/examples/Kuiper.Example1.fst
@@ -26,8 +26,8 @@ fn main (_:unit)
   let gr = gpu_alloc0 #u64 ();
 
   Kuiper.Ref.gpu_memcpy_host_to_device gr r;
-
-  launch_kernel_1 (fun () -> kf gr);
+  with v. assert on gpu_loc (gr |-> v);
+  launch_kernel_1 (fun () -> kf gr #v);
 
   Kuiper.Ref.gpu_memcpy_device_to_host r gr;
 
