src/examples/Kuiper.Example2.fst
@@ -22,6 +22,7 @@ fn main (_:unit)
   returns  _ : u64
   ensures emp
 {
+  Pulse.Lib.Core.on_intro #gpu_loc emp;
   launch_kernel_1 (fun () -> kf ());
   1uL
 }
