src/lib/data/Kuiper.Matrix.fsti
@@ -44,6 +44,8 @@ instance cview_from_clayout
 inline_for_extraction noextract
 val gpu_matrix (et:Type0) (#rows #cols : nat) (l : mlayout rows cols) : Type0
 
+val is_global_matrix (#et:Type0) (#rows #cols : nat) (#l : mlayout rows cols) (g:gpu_matrix et l) : prop
+
 inline_for_extraction noextract
 val from_array
   (#a : Type0)
@@ -65,7 +67,7 @@ val lem_core_from_array
   (#rows #cols : erased nat)
   (#l : mlayout rows cols)
   (g : gpu_matrix et l)
-  : Lemma (ensures from_array l (core g) == g)
+  : Lemma (ensures from_array l (core g) == g /\ (is_global_array (core g) <==> is_global_matrix g))
           [SMTPat (core g)]
 
 val lem_from_array_core
@@ -73,7 +75,7 @@ val lem_from_array_core
   (#rows #cols : erased nat)
   (#l : mlayout rows cols)
   (p : gpu_array et (mlayout_size l))
-  : Lemma (ensures core (from_array l p) == p)
+  : Lemma (ensures core (from_array l p) == p /\ (is_global_matrix (from_array l p) <==> is_global_array p))
           [SMTPat (from_array l p)]
 
 val gpu_matrix_pts_to
@@ -82,6 +84,16 @@ val gpu_matrix_pts_to
   (#[T.exact (`1.0R)] f : perm)
   (em : ematrix et rows cols)
   : slprop
+
+instance
+val is_send_across_global_matrix
+  (#et:Type0)
+  (#rows #cols : nat)
+  (#l : mlayout rows cols)
+  (x: gpu_matrix et l { is_global_matrix x })
+  (#f : perm)
+  (em : ematrix et rows cols)
+  : Pulse.Lib.SendSync.is_send_across gpu_of (gpu_matrix_pts_to x #f em)
 
 (* erased is important for the lens! *)
 unfold
@@ -100,6 +112,21 @@ fn gpu_matrix_pts_to_ref
   (#em : ematrix et rows cols)
   preserves
     gpu_matrix_pts_to g #f em
+  ensures
+    pure (SZ.fits (mlayout_size l))
+
+
+ghost
+fn gpu_matrix_pts_to_ref_located
+  (#et:Type)
+  (#rows #cols : nat)
+  (#l : mlayout rows cols)
+  (g : gpu_matrix et l)
+  (#loc:_)
+  (#f : perm)
+  (#em : ematrix et rows cols)
+  preserves
+    on loc (gpu_matrix_pts_to g #f em)
   ensures
     pure (SZ.fits (mlayout_size l))
 
