src/lib/poly/Kuiper.Poly.HReduce.fst
@@ -434,49 +434,12 @@ let kernel
   kpre =  kpre lena a va vr;
   frame = emp;
 }
-module T = FStar.Tactics
-
-assume
-val rewrite_by_unfolding (p:slprop) (steps:_)
-: stt_ghost unit emp_inames p (fun _ -> norm steps p)
-
-
-ghost fn on_exists_elim u#a #l (#a: Type u#a) (p: a -> slprop)
-  requires on l (exists* x. p x)
-  ensures exists* x. on l (p x)
-{
-  admit()
-  
-  // ghost_impersonate l (on l (exists* x. p x)) (exists* x. on l (p x)) fn _ {
-  //   on_elim (exists* x. p x);
-  //   on_intro (p _);
-  // }
-}
-
-ghost fn on_star_elim #l (p q: slprop)
-  requires on l (p ** q)
-  ensures on l p
-  ensures on l q
-{
-  admit()
-}
-
-
-ghost fn placeless_on_elim (p: slprop) {| placeless p |} l
-  requires on l p
-  ensures p
-  {admit()}
-
-ghost fn on_pure_elim (p:prop) l
-  requires on l (pure p)
-  ensures pure p
-  {admit()}
 
 inline_for_extraction noextract
 fn reduce
   (#et:Type0) {| scalar et, real_like et |}
   (lena : szp { lena < max_threads })
-  (a : gpu_array et lena)
+  (a : gpu_array et lena { is_global_array a })
   (#va : erased (seq et))
   (#vr : erased (seq real) { va %~ vr })
   requires
@@ -490,7 +453,7 @@ fn reduce
 {
   gpu_pts_to_ref_located a; (* recall length, automate *)
   launch_sync (kernel lena a #va #vr);
-  rewrite_by_unfolding
+  reduce_with_steps
     (on gpu_loc (gpu_pts_to_slice_sum a 0 lena va vr))
     [delta_only [`%gpu_pts_to_slice_sum]];
   on_exists_elim _;
